for a cmd in block b that uses id0, if the b is not reachable, typings do not need to check any property of id0, because the b cannot execute at runtime. The old rule still checked if id0 is defined in some block in the unreachable case. This complicated substitution-preserving-WF proofs.
In LAS, we require the stored value dominates the loaded temporary only
when the load's block b is reachable, but allow anything when b is
unreachable. By doing so, the algorithm is simpler w/o checking
reachability. But, in the old typing rules, when b is unreachable, we
still need to find the block that defines the stored value. Although
this is provable, the proof is not clean. So, we changed the wf_operand
rule to check nothing when a block under check is unreachable.

Save point before the same update for phinode.



git-svn-id: https://webdav.seas.upenn.edu/svn/sol/vol@3966 eef5ea85-cc2e-0410-bd84-0fae1f012da8

src3.0/Transforms/id_rhs_val.v
@@ -152,13 +152,16 @@ match v with
     end
 end.
 
-Definition substing_value (f:fdef) (v:value) : Prop :=
+
+Definition substing_value (f:fdef) (v:value) : Prop := True.
+(*
 match v with
 | value_const _ => True
 | value_id vid =>
     In vid (getArgsIDsOfFdef f) \/
-    exists b, lookupBlockViaIDFromFdef f vid = Some b
+    exists b, lookupBlockViaIDFromFdef f vid = Some b)
 end.
+*)
 
 Definition substable_values TD gl (f:fdef) (v1 v2:value) : Prop :=
 substable_value f v1 /\ substing_value f v2 /\ valueDominates f v2 v1 /\
